final commit of overly complex subset type attempt

Analysis.v
@@ -34,6 +34,17 @@ Definition get_fin (i:nat) : option (Vectors.Fin.t 16) :=
 
 Definition ne_ins := { l : list instr | l <> [] }.
 
+Theorem cons_not_nil : forall A (x:A) (l:list A), (x :: l) <> [].
+Proof.
+  discriminate.
+Qed.
+
+Definition get_ne_ins (l:list instr) : option ne_ins :=
+  match l with
+      | [] => None
+      | a :: rest => Some (exist _ (a :: rest) (cons_not_nil _ a rest))
+    end.
+
 Record vm_state : Type := make_state {
   acc : option imm;
   x_reg : option imm;
@@ -41,20 +52,6 @@ Record vm_state : Type := make_state {
   pkt : list (Word.word 32);
   smem : scratch_mem
 }.
-
-Definition change_acc (s:vm_state) (ins:ne_ins) (new_acc:imm) :=
-  make_state (Some new_acc) (x_reg s) ins (pkt s) (smem s).
-
-Definition change_x_reg (s:vm_state) (ins:ne_ins) (new_x:imm) :=
-  make_state (acc s) (Some new_x) ins (pkt s) (smem s).
-
-Definition change_smem (s:vm_state) (ins:ne_ins) (i:nat) (v:Word.word 32) : option vm_state :=
-  match get_fin i with
-    | Some fin =>
-        let new_mem := Vector.replace (smem s) fin (Some v) in
-        Some (make_state (acc s) (x_reg s) ins (pkt s) new_mem)
-    | None => None
-  end.
 
 Inductive end_state : Type :=
   | Ret : Word.word 32 -> end_state
@@ -67,13 +64,27 @@ Inductive state : Type :=
 Definition init_state (ins:ne_ins) : state :=
   ContState (make_state None None ins [] empty_mem).
 
-Print sig.
+Definition change_acc (s:vm_state) (ins:list instr) (new_acc:imm) : state :=
+  match get_ne_ins ins with
+    | None => End (Error "altering acc as last instr")
+    | Some ne_l => 
+        ContState (make_state (Some new_acc) (x_reg s) ne_l (pkt s) (smem s))
+  end.
 
+Definition change_x_reg (s:vm_state) (ins:list instr) (new_x:imm) : state :=
+  match get_ne_ins ins with
+    | None => End (Error "altering acc as last instr")
+    | Some ne_l =>
+        ContState (make_state (acc s) (Some new_x) ne_l (pkt s) (smem s))
+  end.
 
-Theorem cons_not_nil : forall A (x:A) (l:list A), (x :: l) <> [].
-Proof.
-  discriminate.
-Qed.
+Definition change_smem (s:vm_state) (ins:ne_ins) (i:nat) (v:Word.word 32) : option vm_state :=
+  match get_fin i with
+    | Some fin =>
+        let new_mem := Vector.replace (smem s) fin (Some v) in
+        Some (make_state (acc s) (x_reg s) ins (pkt s) new_mem)
+    | None => None
+  end.
 
 Definition skip_n_ni (n:nat) (l:ne_ins) : option ne_ins :=
     match skipn n (` l) with
@@ -88,38 +99,46 @@ Definition jump (s:vm_state) (n:word 32) : state :=
     | None =>
         End (Error "jumped out of bounds")
   end.
-   
+
+Definition ne_hd : forall (l:list instr), l <> [] -> instr.
+  refine (fun l p =>
+  match l return ((l <> []) -> instr) with
+    | [] => fun H => _
+    | (a :: rest) => fun H => a
+  end p).
+Proof.
+  intuition.
+Qed.
 
 Definition step (s:vm_state) : state :=
-  match ` (ins s) with
-    | [] => End (Error "never reached return")
-    | i :: rest =>
-      match i with
-        | SoloInstr s_op =>
-            match s_op with
-              | RetA =>
-                  match acc s with
-                    | None => End (Error "Returned uninitialized acc")
-                    | Some v => End (Ret v)
-                  end
-              | XStoreA =>
-                  match acc s with
-                    | Some acc' =>
-                        ContState (change_x_reg s rest acc')
-                    | None =>
-                        End (Error "storing acc to uninitialized x reg")
-                  end
-              | AStoreX =>
-                  match x_reg s with
-                    | Some x' =>
-                        ContState (change_acc s rest x')
-                    | None =>
-                        End (Error "storing x reg to uninitialized acc")
-                  end
+  let i := ne_hd (` (ins s)) (proj2_sig (ins s)) in
+  let rest := tl (` (ins s)) in
+  match i with
+    | SoloInstr s_op =>
+        match s_op with
+          | RetA =>
+              match acc s with
+                | None => End (Error "Returned uninitialized acc")
+                | Some v => End (Ret v)
+              end
+          | XStoreA =>
+              match acc s with
+                | Some acc' =>
+                    change_x_reg s rest acc'
+                | None =>
+                    End (Error "storing acc to uninitialized x reg")
+              end
+          | AStoreX =>
+              match x_reg s with
+                | Some x' =>
+                    change_acc s rest x'
+                | None =>
+                    End (Error "storing x reg to uninitialized acc")
+              end
               | AddX =>
                         match acc s, x_reg s with
                             | Some acc', Some x' =>
-                                ContState (change_acc s rest ((acc') ^+ x'))
+                                change_acc s rest ((acc') ^+ x')
                             | None, _ =>
                                 End (Error "Adding to uninitialized acc")
                             | _, None =>
@@ -128,7 +147,7 @@ Definition step (s:vm_state) : state :=
                     | SubX =>
                         match acc s, x_reg s with
                             | Some acc', Some x' =>
-                                ContState (change_acc s rest ((acc') ^- x'))
+                                change_acc s rest ((acc') ^- x')
                             | None, _ =>
                                 End (Error "Subtracting to uninitialized acc")
                             | _, None =>
@@ -137,7 +156,7 @@ Definition step (s:vm_state) : state :=
                     | MulX =>
                         match acc s, x_reg s with
                             | Some acc', Some x' =>
-                                ContState (change_acc s rest ((acc') ^* x'))
+                                change_acc s rest ((acc') ^* x')
                             | None, _ =>
                                 End (Error "Multiplying to uninitialized acc")
                             | _, None =>
@@ -148,7 +167,7 @@ Definition step (s:vm_state) : state :=
                     | AndX =>
                         match acc s, x_reg s with
                             | Some acc', Some x' =>
-                                ContState (change_acc s rest ((acc') ^& x'))
+                                change_acc s rest ((acc') ^& x')
                             | None, _ =>
                                 End (Error "And-ing to uninitialized acc")
                             | _, None =>
@@ -157,7 +176,7 @@ Definition step (s:vm_state) : state :=
                     | OrX =>
                         match acc s, x_reg s with
                             | Some acc', Some x' =>
-                                ContState (change_acc s rest ((acc') ^| x'))
+                                change_acc s rest ((acc') ^| x')
                             | None, _ =>
                                 End (Error "Or-ing to uninitialized acc")
                             | _, None =>
@@ -171,35 +190,35 @@ Definition step (s:vm_state) : state :=
                         End (Error "*** fill in ***")
                     | LdLen =>
                         let pkt_len := Word.natToWord 32 (length (pkt s)) in
-                        ContState (change_acc s rest pkt_len)
+                        change_acc s rest pkt_len
                     | LdXLen =>
                         let pkt_len := Word.natToWord 32 (length (pkt s)) in
-                        ContState (change_x_reg s rest pkt_len)
+                        change_x_reg s rest pkt_len
                 end
             | ImmInstr i_op i =>
                 match i_op with
                     | RetK =>
                         End (Ret i)
                     | LdImm =>
-                        ContState (change_acc s rest i)
+                        change_acc s rest i
                     | AddImm =>
                         match acc s with
                             | Some acc' =>
-                                ContState (change_acc s rest ((acc') ^+ i))
+                                change_acc s rest ((acc') ^+ i)
                             | None =>
                                 End (Error "Adding to uninitialized acc")
                         end
                     | SubImm =>
                         match acc s with
                             | Some acc' =>
-                                ContState (change_acc s rest ((acc') ^- i))
+                                change_acc s rest ((acc') ^- i)
                             | None =>
                                 End (Error "Subtracting to uninitialized acc")
                         end
                     | MulImm =>
                         match acc s with
                             | Some acc' =>
-                                ContState (change_acc s rest ((acc') ^* i))
+                                change_acc s rest ((acc') ^* i)
                             | None =>
                                 End (Error "Multiplying to uninitialized acc")
                         end
@@ -208,14 +227,14 @@ Definition step (s:vm_state) : state :=
                     | AndImm =>
                         match acc s with
                             | Some acc' =>
-                                ContState (change_acc s rest ((acc') ^& i))
+                                change_acc s rest ((acc') ^& i)
                             | None =>
                                 End (Error "And-ing to uninitialized acc")
                         end
                     | OrImm =>
                         match acc s with
                             | Some acc' =>
-                                ContState (change_acc s rest ((acc') ^| i))
+                                change_acc s rest ((acc') ^| i)
                             | None =>
                                 End (Error "Or-ing to uninitialized acc")
                         end
@@ -226,14 +245,14 @@ Definition step (s:vm_state) : state :=
                     | Neg =>
                         match acc s with
                             | Some acc' =>
-                                ContState (change_acc s rest (wneg acc'))
+                                change_acc s rest (wneg acc')
                             | None =>
                                 End (Error "Adding to uninitialized acc")
                         end
                     | JmpImm =>
                         jump s i
                     | LdXImm =>
-                        ContState (change_x_reg s rest i)
+                        change_x_reg s rest i
                 end
             | MemInstr m_op m_addr =>
                 match m_op with
@@ -294,16 +313,31 @@ Definition step (s:vm_state) : state :=
                     | JAndImm =>
                         End (Error "*** fill in ***")
                 end
-        end
   end.
 
 Definition size (s:state) : nat :=
   match s with
     | End _ => 0
-    | ContState cs => length (ins cs)
+    | ContState cs => length (` (ins cs))
   end.
 
-Require Coq.Program.Wf.
+Definition t (l:list instr) (p:l <> []) : ne_ins := (exist _ l p).
+Print t.
+
+Lemma impl_subset : forall (l:list instr) (p:l <> []),
+  p -> length l = length (` (exist _ l p)).
+
+Definition is_cs (s:state) : Prop :=
+  match s with
+    | End _ => False
+    | ContState _ => True
+  end.
+
+Lemma cs_gz : forall (s:state), is_cs s -> gt (size s) 0.
+Proof.
+  intros.
+  destruct s.
+  simpl. intuition.
 
 Program Fixpoint prog_eval (s: state) { measure (size s) } : end_state :=
   match s with
@@ -316,8 +350,10 @@ Lemma end_less : forall a b, lt (size (End a)) (size (ContState b)).
 
 Next Obligation.
   induction (step cs).
-  simpl.
+  simpl. 
   destruct cs. simpl.
+  destruct v. simpl.
+  Case .
 
 (*
    Used to prove that offsets stay on word (and hence instruction)
